Prove equivalence with flags i, m and s modulo a few admits on begin/end input anchors

Semantics/Chars.v
@@ -1,8 +1,8 @@
 Require Import List Lia.
 Import ListNotations.
-From Linden Require Import Utils Parameters.
+From Linden Require Import Utils Parameters LWParameters CharSet.
 Import Utils.List.
-From Warblre Require Import Base Typeclasses RegExpRecord.
+From Warblre Require Import Base Typeclasses RegExpRecord Semantics Result Errors.
 
 (** * Characters and Strings  *)
 
@@ -10,18 +10,10 @@ Section Chars.
   Context {params: LindenParameters}.
   Context (rer: RegExpRecord).
 
-  Definition string := list Character.
-
   (* In the semantics, the input string is represented with both the next characters to read
    and the reversed list of previously read characters (in case we change direction for a lookbehind) *)
   Inductive input : Type :=
   | Input (next: string) (pref: string).
-
-  Definition string_eq_dec : forall (x y : string), { x = y } + { x <> y }.
-  Proof.
-    decide equality. apply Character.eq_dec.
-  Defined.
-  #[export] Instance string_EqDec: EqDec string := EqDec.make string string_eq_dec.
 
   Definition input_eq_dec: forall (i1 i2: input), { i1 = i2 } + { i1 <> i2 }.
   Proof. decide equality; apply string_eq_dec. Defined.
@@ -85,8 +77,14 @@ Section Chars.
   Qed.
 
 
+  Definition wordCharacters (rer: RegExpRecord): CharSet :=
+    match Semantics.wordCharacters rer with
+    | Success cs => cs
+    | Error _ => Characters.ascii_word_characters
+    end.
+
   (* Deciding whether a character is a word character, to check for word boundaries and for character classes \w and \W *)
-  Definition word_char c := inb_canonicalized c Character.ascii_word_characters.
+  Definition word_char c := CharSet.contains (wordCharacters rer) c.
 
   (* Lemma for boolean version of In *)
   Lemma char_all_inb: forall c, inb c Character.all = true.
@@ -104,33 +102,50 @@ Section Chars.
   | CdAll
   | CdSingle (c: Character)
   | CdDigits
+  | CdNonDigits
   | CdWhitespace
+  | CdNonWhitespace
   | CdWordChar
+  | CdNonWordChar
   | CdUnicodeProp (p: Property)
+  | CdNonUnicodeProp (p: Property)
   | CdInv (cd: char_descr)
   | CdRange (l h: Character)
   | CdUnion (cd1 cd2: char_descr).
+
+  (* Whether dot matches a character *)
+  Definition dot_matches (dotAll: bool) (c: Character): bool :=
+    if dotAll then
+      true
+    else
+      CharSetExt.exist_canonicalized rer (CharSetExt.remove_all Characters.all Characters.line_terminators) c.
   
-  Fixpoint char_match (c: Character) (cd: char_descr): bool :=
+  Fixpoint char_match' (ccan: Character) (cd: char_descr): bool :=
     match cd with
     | CdEmpty => false
     | CdDot => 
-        if RegExpRecord.dotAll rer then
-          true
-        else
-          negb (inb_canonicalized c Character.line_terminators)
+        dot_matches (RegExpRecord.dotAll rer) ccan
     | CdAll => true
-    | CdSingle c' => Character.canonicalize rer c == Character.canonicalize rer c'
-    | CdDigits => inb_canonicalized c Character.digits
-    | CdWhitespace => inb_canonicalized c Character.white_spaces || inb_canonicalized c Character.line_terminators
-    | CdWordChar => inb_canonicalized c Character.ascii_word_characters (* Temporary; at the end, we'd like to use a rer *)
-    | CdUnicodeProp p => inb_canonicalized c (Property.code_points_for p)
-    | CdInv cd' => negb (char_match c cd')
+    | CdSingle c' => ccan == Character.canonicalize rer c'
+    | CdDigits => CharSetExt.exist_canonicalized rer Characters.digits ccan
+    | CdNonDigits => CharSetExt.exist_canonicalized rer (CharSetExt.remove_all Characters.all Characters.digits) ccan
+    | CdWhitespace => CharSetExt.exist_canonicalized rer (CharSet.union Characters.white_spaces Characters.line_terminators) ccan
+    | CdNonWhitespace => CharSetExt.exist_canonicalized rer (CharSetExt.remove_all Characters.all (CharSet.union Characters.white_spaces Characters.line_terminators)) ccan
+    | CdWordChar => CharSetExt.exist_canonicalized rer (wordCharacters rer) ccan
+    | CdNonWordChar => CharSetExt.exist_canonicalized rer (CharSetExt.remove_all Characters.all (wordCharacters rer)) ccan
+    | CdUnicodeProp p => CharSetExt.exist_canonicalized rer (CharSetExt.from_list (Property.code_points_for p)) ccan
+    | CdNonUnicodeProp p => CharSetExt.exist_canonicalized rer (CharSetExt.remove_all Characters.all (CharSetExt.from_list (Property.code_points_for p))) ccan
+    | CdInv cd' => negb (char_match' ccan cd')
     | CdRange l h =>
-        let charSet := List.filter (fun x => (Character.numeric_value l <=? Character.numeric_value x) && (Character.numeric_value x <=? Character.numeric_value h))%bool Character.all in
-        inb_canonicalized c charSet
-    | CdUnion cd1 cd2 => char_match c cd1 || char_match c cd2
+        let i := Character.numeric_value l in
+        let j := Character.numeric_value h in
+        let charSet := CharSetExt.range (Character.from_numeric_value i) (Character.from_numeric_value j) in
+        CharSetExt.exist_canonicalized rer charSet ccan
+    | CdUnion cd1 cd2 => char_match' ccan cd1 || char_match' ccan cd2
     end.
+
+  Definition char_match (c: Character) (cd: char_descr) :=
+    char_match' (Character.canonicalize rer c) cd.
 
 
   Lemma single_match:
@@ -140,7 +155,7 @@ Section Chars.
   Qed.
 
   Definition char_descr_eq_dec : forall (cd1 cd2: char_descr), { cd1 = cd2 } + { cd1 <> cd2 }.
-  Proof. decide equality; try apply Character.eq_dec. apply Property.unicode_property_eqdec. Defined.
+  Proof. decide equality; try apply Character.eq_dec; try apply Property.unicode_property_eqdec. Defined.
 
 
   (** * Reading Characters in the String *)
