WarblreEquiv/CharDescrCharSet.v
@@ -9,31 +9,20 @@ Local Open Scope result_flow.
 Section CharDescrCharSet.
   Context {params: LindenParameters}.
   Context (rer: RegExpRecord).
-
-  (* In CharSet equivalences, we do not want to ignore case. This is so that
-  each character descriptor is made equivalent to the CharSet passed to
-  Semantics.characterSetMatcher for the corresponding Warblre character
-  descriptor. *)
-  Definition rer_noi : RegExpRecord := {|
-    RegExpRecord.ignoreCase := false;
-    RegExpRecord.multiline := RegExpRecord.multiline rer;
-    RegExpRecord.dotAll := RegExpRecord.dotAll rer;
-    RegExpRecord.unicode := tt;
-    RegExpRecord.capturingGroupsCount := RegExpRecord.capturingGroupsCount rer
-  |}.
   
   Definition equiv_cd_charset (cd: char_descr) (charset: CharSet) :=
-    forall c: Character, char_match rer_noi c cd = CharSet.contains charset c.
+    forall c: Character, char_match rer c cd = CharSet.exist_canonicalized rer charset (Character.canonicalize rer c).
 
   (* Lemma for character descriptor inversion *)
-  Lemma equiv_cd_inv:
+  (* Should not be needed *)
+  (*Lemma equiv_cd_inv:
     forall cd s, equiv_cd_charset cd s -> equiv_cd_charset (CdInv cd) (CharSet.remove_all Characters.all s).
   Proof.
     intros cd s H c. specialize (H c).
     simpl. apply Bool.eq_true_iff_eq.
     rewrite CharSetExt.remove_all_contains. rewrite H.
     setoid_rewrite contains_all. simpl. reflexivity.
-  Qed.
+  Qed.*)
 
   (* Lemma for character descriptor union *)
   Lemma equiv_cd_union:
@@ -41,50 +30,58 @@ Section CharDescrCharSet.
       equiv_cd_charset cd1 s1 -> equiv_cd_charset cd2 s2 ->
       equiv_cd_charset (CdUnion cd1 cd2) (CharSet.union s1 s2).
   Proof.
-    intros cd1 cd2 s1 s2 Hequiv1 Hequiv2 c.
-    simpl. setoid_rewrite CharSetExt.union_contains. rewrite Hequiv1. rewrite Hequiv2. reflexivity.
-  Qed.
-
-  (* Inversion lemma for singletons *)
-  Lemma equiv_cd_singleton_invn:
-    forall c s,
-      equiv_cd_charset (CdSingle c) s -> CharSetExt.Equal s (CharSet.singleton c).
-  Proof.
-    intros c s Hequiv chr.
-    specialize (Hequiv chr). simpl in Hequiv.
-    do 2 rewrite canonicalize_casesenst in Hequiv by reflexivity.
-    apply Bool.eq_iff_eq_true in Hequiv.
-    rewrite CharSetExt.contains_spec in Hequiv.
-    rewrite Typeclasses.EqDec.inversion_true in Hequiv.
-    setoid_rewrite CharSetExt.singleton_spec. rewrite <- Hequiv. split; congruence.
+    intros cd1 cd2 s1 s2 Hequiv1 Hequiv2 c. unfold char_match.
+    simpl. rewrite CharSetExt.exist_canonicalized_equiv.
+    apply Bool.eq_iff_eq_true. rewrite CharSetExt.exist_iff.
+    setoid_rewrite CharSetExt.union_contains.
+    split.
+    - intro H. apply Bool.orb_prop in H. destruct H.
+      + specialize (Hequiv1 c). setoid_rewrite H in Hequiv1.
+        symmetry in Hequiv1. rewrite CharSet.exist_canonicalized_equiv in Hequiv1.
+        setoid_rewrite CharSetExt.exist_iff in Hequiv1.
+        setoid_rewrite Bool.orb_true_iff. firstorder.
+      + specialize (Hequiv2 c). setoid_rewrite H in Hequiv2.
+        symmetry in Hequiv2. rewrite CharSet.exist_canonicalized_equiv in Hequiv2.
+        setoid_rewrite CharSetExt.exist_iff in Hequiv2.
+        setoid_rewrite Bool.orb_true_iff. firstorder.
+    - setoid_rewrite Bool.orb_true_iff. intros [c0 [Hcontains Hcanonicalize]].
+      destruct Hcontains as [Hcontains | Hcontains].
+      + left. specialize (Hequiv1 c). setoid_rewrite Hequiv1.
+        setoid_rewrite CharSetExt.exist_canonicalized_equiv.
+        rewrite CharSetExt.exist_iff. exists c0. auto.
+      + right. specialize (Hequiv2 c). setoid_rewrite Hequiv2.
+        setoid_rewrite CharSetExt.exist_canonicalized_equiv.
+        rewrite CharSetExt.exist_iff. exists c0. auto.
   Qed.
 
   (* Lemmas for various character descriptors *)
   Lemma equiv_cd_empty:
     equiv_cd_charset CdEmpty CharSet.empty.
   Proof.
-    intro c. simpl. setoid_rewrite CharSetExt.empty_contains. reflexivity.
+    intro c. unfold char_match. simpl.
+    rewrite CharSetExt.exist_canonicalized_equiv.
+    symmetry. apply Bool.not_true_is_false.
+    intro ABS. rewrite CharSetExt.exist_iff in ABS.
+    destruct ABS as [c0 [ABS _]].
+    rewrite CharSetExt.empty_contains in ABS. discriminate ABS.
   Qed.
 
   Lemma equiv_cd_digits:
     equiv_cd_charset CdDigits Characters.digits.
   Proof.
-    intro c. simpl. rewrite inb_canonicalized_casesenst by reflexivity.
-    unfold Characters.digits. now setoid_rewrite CharSetExt.from_list_contains_inb.
+    intro c. simpl. reflexivity.
   Qed.
 
   Lemma equiv_cd_whitespace:
     equiv_cd_charset CdWhitespace (CharSet.union Characters.white_spaces Characters.line_terminators).
   Proof.
-    intro c. simpl. do 2 rewrite inb_canonicalized_casesenst by reflexivity.
-    unfold Characters.white_spaces, Characters.line_terminators. setoid_rewrite CharSetExt.union_contains. now setoid_rewrite CharSetExt.from_list_contains_inb.
+    intro c. simpl. reflexivity.
   Qed.
 
   Lemma equiv_cd_wordchar:
-    equiv_cd_charset CdWordChar Characters.ascii_word_characters.
+    equiv_cd_charset CdWordChar (Chars.wordCharacters rer).
   Proof.
-    intro c. simpl. rewrite inb_canonicalized_casesenst by reflexivity.
-    unfold Characters.ascii_word_characters. now setoid_rewrite CharSetExt.from_list_contains_inb.
+    intro c. simpl. reflexivity.
   Qed.
 
   Lemma equiv_cd_range:
@@ -92,87 +89,85 @@ Section CharDescrCharSet.
       Character.numeric_value cl <= Character.numeric_value ch ->
       equiv_cd_charset (CdRange cl ch) (CharSet.range cl ch).
   Proof.
-    intros cl ch Hle c. simpl.
-    rewrite inb_canonicalized_casesenst by reflexivity.
-    apply Bool.eq_true_iff_eq.
-    rewrite Utils.List.inb_spec, CharSetExt.contains_spec, CharSetExt.range_spec.
-    rewrite List.filter_In, Bool.andb_true_iff, PeanoNat.Nat.leb_le, PeanoNat.Nat.leb_le.
-    pose proof char_all_in c. tauto.
+    intros cl ch Hle c. unfold char_match. simpl.
+    do 2 rewrite Character.numeric_pseudo_bij. reflexivity.
   Qed.
 
   Lemma equiv_cd_dot_dotAll:
     RegExpRecord.dotAll rer = true ->
     equiv_cd_charset CdDot Characters.all.
   Proof.
-    intros HdotAll c. simpl. rewrite HdotAll. symmetry. apply contains_all.
+    intros HdotAll c. unfold char_match. simpl. unfold dot_matches. rewrite HdotAll. symmetry.
+    rewrite CharSetExt.exist_canonicalized_equiv, CharSetExt.exist_iff.
+    exists c. split.
+    - apply contains_all.
+    - apply EqDec.reflb.
   Qed.
 
   Lemma equiv_cd_dot_noDotAll:
     RegExpRecord.dotAll rer = false ->
     equiv_cd_charset CdDot (CharSet.remove_all Characters.all Characters.line_terminators).
   Proof.
-    intros HnoDotAll c. simpl. rewrite HnoDotAll.
-    rewrite inb_canonicalized_casesenst by reflexivity.
-    apply Bool.eq_true_iff_eq.
-    rewrite CharSetExt.remove_all_contains. 
-    setoid_rewrite contains_all. simpl.
-    unfold Characters.line_terminators. setoid_rewrite CharSetExt.from_list_contains_inb.
+    intros HnoDotAll c. unfold char_match. simpl. unfold dot_matches. rewrite HnoDotAll.
     reflexivity.
   Qed.
     
   Lemma equiv_cd_single:
     forall c, equiv_cd_charset (CdSingle c) (CharSet.singleton c).
   Proof.
-    intros c chr. simpl. do 2 rewrite canonicalize_casesenst by reflexivity. symmetry. apply CharSetExt.contains_singleton.
+    intros c chr. unfold char_match. simpl.
+    rewrite CharSetExt.exist_canonicalized_equiv. rewrite CharSetExt.singleton_exist.
+    destruct EqDec.eqb eqn:H.
+    - rewrite EqDec.inversion_true in H. symmetry. rewrite H. apply EqDec.reflb.
+    - symmetry. apply Bool.not_true_is_false. intro ABS.
+      rewrite EqDec.inversion_true in ABS. rewrite ABS, EqDec.reflb in H. discriminate H.
   Qed.
 
   Lemma equiv_cd_unicodeprop:
     forall p, equiv_cd_charset (CdUnicodeProp p) (CharSetExt.from_list (Property.code_points_for p)).
   Proof.
-    intros p c. simpl. rewrite inb_canonicalized_casesenst by reflexivity. now setoid_rewrite CharSetExt.from_list_contains_inb.
+    intros p c. unfold char_match. simpl. reflexivity.
   Qed.
 
   (* Lemma for CharacterClassEscapes *)
+  (* TODO From here *)
   Lemma equiv_cd_CharacterClassEscape:
-    forall esc cd rer,
-      RegExpRecord.ignoreCase rer = false ->
+    forall esc cd,
       equiv_CharacterClassEscape esc cd ->
       exists a, Semantics.compileToCharSet_ClassAtom (ClassEsc (CCharacterClassEsc esc)) rer = Success a /\
              equiv_cd_charset cd a.
   Proof.
-    intros esc cd rer Hcasesenst Hequiv.
+    intros esc cd Hequiv.
     inversion Hequiv as [Heqesc Heqcd | Heqesc Heqcd | Heqesc Heqcd | Heqesc Heqcd | Heqesc Heqcd | Heqesc Heqcd | p Heqesc Heqcd | p Heqesc Heqcd ]; simpl; unfold Coercions.Coercions.wrap_CharSet; eexists; split; try solve[reflexivity].
     - apply equiv_cd_digits.
-    - apply equiv_cd_inv. apply equiv_cd_digits.
+    - unfold equiv_cd_charset. reflexivity.
     - apply equiv_cd_whitespace.
-    - apply equiv_cd_inv. apply equiv_cd_whitespace.
-    - pose proof wordCharacters_casesenst_eq rer Hcasesenst. unfold Semantics.wordCharacters, Coercions.Coercions.wrap_CharSet in H. simpl in H.
-      injection H as H. setoid_rewrite H. apply equiv_cd_wordchar.
-    - apply equiv_cd_inv. pose proof wordCharacters_casesenst_eq rer Hcasesenst. unfold Semantics.wordCharacters, Coercions.Coercions.wrap_CharSet in H. simpl in H.
-      injection H as H. setoid_rewrite H. apply equiv_cd_wordchar.
+    - unfold equiv_cd_charset. reflexivity.
+    - apply equiv_cd_wordchar.
+    - unfold equiv_cd_charset. reflexivity.
     - apply equiv_cd_unicodeprop.
-    - apply equiv_cd_inv. apply equiv_cd_unicodeprop.
+    - unfold equiv_cd_charset. reflexivity.
   Qed.
 
   (* Lemma for ControlEscapes *)
   Lemma equiv_cd_ControlEscape:
-    forall esc cd rer,
+    forall esc cd,
       equiv_ControlEscape esc cd ->
       exists a, Semantics.compileToCharSet_ClassAtom (ClassEsc (CCharacterEsc (ControlEsc esc))) rer = Success a /\
              equiv_cd_charset cd a.
   Proof.
-    intros esc cd rer Hequiv.
+    intros esc cd Hequiv.
     inversion Hequiv; simpl; unfold Coercions.Coercions.wrap_CharSet; eexists; split; try solve[reflexivity]; unfold Numeric.nat_to_nni; rewrite Character.numeric_pseudo_bij; apply equiv_cd_single.
   Qed.
 
   (* Lemma for CharacterEscapes *)
   Lemma equiv_cd_CharacterEscape:
-    forall esc cd rer,
+    forall esc cd,
       equiv_CharacterEscape esc cd ->
       exists a, Semantics.compileToCharSet_ClassAtom (ClassEsc (CCharacterEsc esc)) rer = Success a /\
              equiv_cd_charset cd a.
   Proof.
-    intros esc cd rer Hequiv. inversion Hequiv as [esc0 cd0 Hequiv' Heqesc Heqcd0 | l cd0 Hequiv' Heqesc Heqcd0 | Heqesc Heqcd | d1 d2 Heqesc Heqcd | c Heqesc Heqcd | head tail Heqesc Heqcd | hex Heqesc Heqcd | c Heqesc Heqcd].
+    intros esc cd Hequiv. inversion Hequiv as [esc0 cd0 Hequiv' Heqesc Heqcd0 | l cd0 Hequiv' Heqesc Heqcd0 | Heqesc Heqcd | d1 d2 Heqesc Heqcd | c Heqesc Heqcd | head tail Heqesc Heqcd | hex Heqesc Heqcd | c Heqesc Heqcd].
     - apply equiv_cd_ControlEscape. assumption.
     - inversion Hequiv' as [l0 i Heqi Heql0 Heqcd]. subst cd0 l0.
       simpl. rewrite <- Heqi.
@@ -194,13 +189,12 @@ Section CharDescrCharSet.
 
   (* Lemma for ClassEscapes *)
   Lemma equiv_cd_ClassEscape:
-    forall esc cd rer,
-      RegExpRecord.ignoreCase rer = false ->
+    forall esc cd,
       equiv_ClassEscape esc cd ->
       exists a, Semantics.compileToCharSet_ClassAtom (ClassEsc esc) rer = Success a /\
              equiv_cd_charset cd a.
   Proof.
-    intros esc cd rer Hcasesenst Hequiv. inversion Hequiv as [Heqesc Heqcd | Heqesc Heqcd | |].
+    intros esc cd Hequiv. inversion Hequiv as [Heqesc Heqcd | Heqesc Heqcd | |].
     - simpl. unfold Coercions.Coercions.wrap_CharSet. eexists. split.
       + reflexivity.
       + unfold Numeric.nat_to_nni. rewrite Character.numeric_pseudo_bij. apply equiv_cd_single.
@@ -213,43 +207,52 @@ Section CharDescrCharSet.
 
   (* Lemmas for ClassRanges *)
   Lemma equiv_cd_ClassAtom:
-    forall ca cacd rer,
-      RegExpRecord.ignoreCase rer = false ->
+    forall ca cacd,
       equiv_ClassAtom ca cacd ->
       exists a, Semantics.compileToCharSet_ClassAtom ca rer = Success a /\ equiv_cd_charset cacd a.
   Proof.
-    intros ca cacd rer Hcasesenst Hequiv.
+    intros ca cacd Hequiv.
     inversion Hequiv as [c Heqca Heqcacd | esc cd Hequiv' Heqca Heqcacd].
     - simpl. unfold Coercions.Coercions.wrap_CharSet. eexists. split. + reflexivity. + apply equiv_cd_single.
     - apply equiv_cd_ClassEscape; assumption.
   Qed.
 
+  Lemma equiv_ClassAtom_single_charset:
+    forall (a: ClassAtom) (c: Character),
+      equiv_ClassAtom a (CdSingle c) ->
+      Semantics.compileToCharSet_ClassAtom a rer = Success (CharSet.singleton c).
+  Proof.
+    intros a c EQUIV. inversion EQUIV; subst.
+    - simpl. reflexivity.
+    - inversion H; subst.
+      + simpl. unfold Numeric.nat_to_nni. rewrite Character.numeric_pseudo_bij. reflexivity.
+      + simpl. unfold Numeric.nat_to_nni. rewrite Character.numeric_pseudo_bij. reflexivity.
+      + inversion H0.
+      + inversion H0; subst; simpl; unfold Numeric.nat_to_nni; try rewrite Character.numeric_pseudo_bij; try reflexivity.
+        * inversion H1; subst; simpl; rewrite Character.numeric_pseudo_bij; reflexivity.
+        * inversion H1; subst. reflexivity.
+  Qed.
 
   Lemma equiv_cd_ClassRanges:
-    forall crs cd rer,
-      RegExpRecord.ignoreCase rer = false ->
+    forall crs cd,
       equiv_ClassRanges crs cd ->
       exists a, Semantics.compileToCharSet crs rer = Success a /\
              equiv_cd_charset cd a.
   Proof.
-    intros crs cd rer Hcasesenst Hequiv.
+    intros crs cd Hequiv.
     induction Hequiv as [|ca cacd t tcd Hequiv' Hequiv IH | l h cl ch t tcd Hequivl Hequivh Hl_le_h Hequiv IH].
     - simpl. unfold Coercions.Coercions.wrap_CharSet.
       eexists. split. + reflexivity. + apply equiv_cd_empty.
-    - simpl. pose proof equiv_cd_ClassAtom ca cacd rer Hcasesenst Hequiv' as [A [HeqA Hequivatom]].
+    - simpl. pose proof equiv_cd_ClassAtom ca cacd Hequiv' as [A [HeqA Hequivatom]].
       rewrite HeqA. simpl.
       destruct IH as [B [HeqB IH]]. rewrite HeqB. simpl.
       unfold Coercions.Coercions.wrap_CharSet. eexists. split. + reflexivity. + now apply equiv_cd_union.
     - simpl.
-      pose proof equiv_cd_ClassAtom l (CdSingle cl) rer Hcasesenst Hequivl as [A [HeqA Hequivatoml]].
-      pose proof equiv_cd_ClassAtom h (CdSingle ch) rer Hcasesenst Hequivh as [B [HeqB Hequivatomh]].
-      rewrite HeqA, HeqB. simpl.
+      rewrite equiv_ClassAtom_single_charset with (c := cl) by auto.
+      rewrite equiv_ClassAtom_single_charset with (c := ch) by auto.
+      simpl.
       destruct IH as [C [HeqC IH]]. rewrite HeqC. simpl.
-      unfold Semantics.characterRange.
-      pose proof equiv_cd_singleton_invn cl A Hequivatoml as HAsingleton.
-      pose proof equiv_cd_singleton_invn ch B Hequivatomh as HBsingleton.
-      rewrite <- CharSetExt.canonicity in HAsingleton, HBsingleton.
-      rewrite HAsingleton, HBsingleton. do 2 rewrite CharSet.singleton_size. simpl.
+      unfold Semantics.characterRange. setoid_rewrite CharSet.singleton_size. simpl.
       do 2 rewrite CharSetExt.singleton_unique. simpl.
       pose proof Hl_le_h as Hl_le_h'. rewrite <- PeanoNat.Nat.leb_le in Hl_le_h'. rewrite Hl_le_h'. simpl.
       unfold Coercions.Coercions.wrap_CharSet. eexists. split.
