Semantics/StrictSuffix.v
@@ -1,4 +1,4 @@
-From Linden Require Import Chars Parameters.
+From Linden Require Import Chars Parameters LWParameters.
 From Warblre Require Import Base Parameters.
 From Coq Require Import List Lia.
 Import ListNotations.
